message

TAPLFormalization/02-lambda/AST.lean
@@ -1,26 +1,64 @@
-import Mathlib.Data.Nat.Notation
+import Mathlib.Data.Finset.Basic
 
 inductive LambdaTerm where
   | var (name : String) : LambdaTerm
   | abs (arg : String) (body : LambdaTerm) : LambdaTerm
   | app (t₁ t₂ : LambdaTerm) : LambdaTerm
+  deriving DecidableEq
 
-def FV : LambdaTerm → Std.HashSet String
-  | .var x => .ofList [x]
+-- 1. Use Finset instead of Std.HashSet for seamless interaction with Prop
+def FV : LambdaTerm → Finset String
+  | .var x => {x}
   | .abs arg body => (FV body).erase arg
-  | .app t₁ t₂ => (FV t₁).union (FV t₂)
+  | .app t₁ t₂ => (FV t₁) ∪ (FV t₂)
 
 inductive IndexedTerm where
   | freeV (name : String) : IndexedTerm
   | boundV (index : ℕ) : IndexedTerm
   | app (t₁ t₂ : IndexedTerm) : IndexedTerm
   | abs (body : IndexedTerm) : IndexedTerm
+  deriving DecidableEq
 
-def removeNames' (depth : ℕ) (levels : Std.HashMap String ℕ) : LambdaTerm → IndexedTerm
-  | .var name => match levels[name]? with
+-- 2. Define the extensional Environment as a pure function
+@[simp]
+def Env := String → Option ℕ
+
+@[simp]
+def Env.empty : Env :=
+  fun _ => none
+@[simp]
+def Env.insert (env : Env) (k : String) (v : ℕ) : Env :=
+  fun x => if x = k then some v else env x
+@[simp]
+def Env.erase (env : Env) (k : String) : Env := fun x => if x = k then none else env x
+@[simp]
+lemma Env.ext (env₁ env₂ : Env) (h : ∀ x, env₁ x = env₂ x) : env₁ = env₂ := by
+  funext x
+  exact h x
+
+@[simp]
+def removeNames' (depth : ℕ) (levels : Env) : LambdaTerm → IndexedTerm
+  | .var name => match levels name with
     | .some k => .boundV k
     | .none => .freeV name
   | .abs arg body => .abs (removeNames' (depth + 1) (levels.insert arg depth) body)
   | .app t₁ t₂ => .app (removeNames' depth levels t₁) (removeNames' depth levels t₂)
 
-def removeNames := removeNames' 0 ∅
+@[simp]
+def LambdaTerm.Subst (x : String) (y : String) : LambdaTerm → LambdaTerm
+  | var t => if t = x then var y else if t=y then var x else var t
+  | app v w => app (v.Subst x y) (w.Subst x y)
+  | abs u t =>
+      if u = x then abs y (t.Subst x y)
+      else if u = y then abs x (t.Subst x y)
+      else abs u (t.Subst x y)
+
+inductive Alpha : LambdaTerm → LambdaTerm → Prop
+  | var {x : String} : Alpha (.var x) (.var x)
+  | app {v v' w w' : LambdaTerm} : Alpha v v' → Alpha w w' → Alpha (.app v w) (.app v' w')
+  | abs {x x' : String} {t t' : LambdaTerm} :
+      (x ∉ FV t'∨ x=x') → Alpha t (t'.Subst x x') → Alpha (.abs x t) (.abs x' t')
+
+
+def removeNames : LambdaTerm → IndexedTerm :=
+  removeNames' 0 Env.empty
